finish proof that derive commutes

Validator/Expr/IfExpr.lean
@@ -10,12 +10,22 @@ abbrev IfExprs α := List (IfExpr α)
 
 namespace IfExpr
 
-def eval [BEq α] [DecidableEq α] (ifExpr: IfExpr α) (t: α): Expr α :=
+def eval {α: Type} [DecidableEq α] (ifExpr: IfExpr α) (t: α): Expr α :=
   match ifExpr with
   | IfExpr.mk cnd thn els =>
     if Pred.eval cnd t
     then thn
     else els
 
-def evals [BEq α] [DecidableEq α] (ifExprs: IfExprs α) (t: α): List (Expr α) :=
+def evals {α: Type} [DecidableEq α] (ifExprs: IfExprs α) (t: α): List (Expr α) :=
   List.map (fun x => eval x t) ifExprs
+
+theorem evals_nil_is_nil {α: Type} [DecidableEq α] (a: α):
+  evals [] a = [] := by
+  unfold evals
+  simp
+
+theorem evals_concat_is_concat {α: Type} [DecidableEq α] (xs ys: IfExprs α) (a: α):
+  evals (xs ++ ys) a = evals xs a ++ evals ys a := by
+  unfold evals
+  simp
