Validator/Derive/Enter.lean
@@ -20,5 +20,15 @@ def enter (x: Expr α) (res: IfExprs α := []): IfExprs α :=
 def deriveEnter (xs: Exprs α): IfExprs α :=
   List.flatten (List.map Enter.enter xs)
 
+theorem deriveEnter_nil_is_nil {α: Type u}:
+  @deriveEnter α [] = [] := by
+  unfold deriveEnter
+  simp
+
+theorem deriveEnter_cons_is_concat {α: Type u} (x: Expr α) (xs: Exprs α):
+  deriveEnter (x::xs) = (deriveEnter [x]) ++ (deriveEnter xs) := by
+  unfold deriveEnter
+  simp
+
 class DeriveEnter (m: Type -> Type u) (α: outParam Type)  where
   deriveEnter (xs: Exprs α): m (IfExprs α)
